\documentclass[12pt]{article}
\usepackage[a4paper]{geometry}

\usepackage{commath}

\usepackage[spanish]{babel}
\selectlanguage{spanish}
\usepackage[utf8]{inputenc}


%% Definitions of operators 
\newcommand{\ii}{\mathrm i}
\newcommand{\ee}{\mathrm e}
\DeclareMathOperator{\re}{Re}
\DeclareMathOperator{\im}{Im}

\begin{document}


\noindent H.Rafeiro \hfill Variable Compleja \hfill Lección 1

\begin{enumerate}
	\item Localizar vectorialmente los números $z_1+z_2$ y $z_1-z_2$, donde
		\begin{enumerate}
			\item $z_1=2\ii$, $z_2= \frac{2}{3}-\ii$;
			\item $z_1=(-3,1)$, $z_2=(1,4)$;
			\item $z_1= x+\ii y$, $z_2= x_1-\ii y_1$.
		\end{enumerate}

	\item Verificar que
		\begin{enumerate}
			\item $\left( \sqrt 2-\ii \right)-\ii \left( 1-\sqrt 2\ii \right)=-2\ii$.
			\item $ \frac{1+2\ii}{3-4\ii} + \frac{2-\ii}{5\ii}= -\frac{2}{5}$
			\item $\frac{5\ii}{(1-\ii)(2-\ii)(3-\ii)}= -\frac{1}{2}$
			\item $(1-\ii)^4=-4$.
		\end{enumerate}
	\item Reducir a la forma $x+\ii y$:
		\begin{enumerate}
			\item  $\left( 1-5\ii \right)^2 -4\ii$;
			\item $-\ii \left( -1 +\ii \right)+2$;
			\item $\left( 3+\ii \right)\left( 1-11\ii \right)$;
			\item $(\sqrt{2}-\ii \sqrt{5}) (\sqrt{5}+\ii \sqrt{2})$  
			\item $\frac{3-4\ii}{2\ii}$;
			\item $\frac{2+5\ii}{-1+\ii \sqrt{3}}$;
			\item $\frac{\left( 2-2\ii \right)^2}{1+\ii}$;
			\item $\frac{z-\bar{z}\ii}{\bar z-z\ii}$
		\end{enumerate}
	\item Probar que
		\begin{enumerate}
			\item $\re (\ii z)= -\im (z)$; 
			\item $\left( 1+z \right)^2=1 + 2z+z^2$;
			\item Si $z_1z_2=0$, entonces $z_1=0$ o $z_2=0$;
			\item $z_1-z_2= \bar {z_1}-\bar{z_2}$;
			\item $z_1z_2= \bar{z_1} \bar {z_2}$;
			\item $\omega= \frac{1}{2} \left( -1-\sqrt{3}\ii \right)$ satisface
				\begin{enumerate}
					\item $\omega^2+\omega+1=0$;
					\item $\omega^3=1$.
				\end{enumerate}
		\end{enumerate}
\end{enumerate}

\end{document}
